theories/clang/lib/spawn.v
@@ -1,1 +1,0 @@
-From iris_c.clang Require Import logic notations tactics.
