theories/tests/spawn.v
@@ -1,0 +1,17 @@
+From iris_c.clang Require Import logic notations tactics.
+From iris_c.clang.lib Require Import lock.
+From iris_c.lib Require Import int.
+
+Section test.
+  Context `{clangG Σ}.
+
+  Definition x : ident := 1.
+  Definition r : ident := 2.
+  Definition l : ident.
+  
+  Definition add: expr :=
+    lock l
+    r <- vtrue.
+
+  Lemma add_spec:
+    r ↦ 
